fstar/Impl.NeedSchr.fst
@@ -1,0 +1,179 @@
+module Impl.NeedSchr
+
+module U8 = FStar.UInt8
+module U32 = FStar.UInt32
+
+module S = FStar.Seq
+module B = LowStar.Buffer
+module M = LowStar.Modifies
+module ST = FStar.HyperStack.ST
+
+module Spec = Spec.NeedSchr
+
+open FStar.HyperStack.ST
+open LowStar.BufferOps
+
+// open Lib.RandomBuffer.System
+// open Hacl.NaCl
+
+// From https://fstarlang.github.io/lowstar/html/ExampleMemCpy.html
+let slice_plus_one #a (s1 s2: S.seq a) (i: nat): Lemma
+    (requires (
+        i < S.length s1 /\
+        i < S.length s2 /\
+        S.equal (S.slice s1 0 i) (S.slice s2 0 i) /\
+        S.index s1 i == S.index s2 i))
+    (ensures (
+        S.equal (S.slice s1 0 (i + 1)) (S.slice s2 0 (i + 1))))
+    [ SMTPat (S.slice s1 0 (i + 1)); SMTPat (S.slice s2 0 (i + 1)) ]
+=
+    let x = S.index s1 i in
+    let s1' = S.append (S.slice s1 0 i) (S.cons x S.empty) in
+    let s2' = S.append (S.slice s2 0 i) (S.cons x S.empty) in
+    assert (S.equal s1' (S.slice s1 0 (i + 1)));
+    assert (S.equal s2' (S.slice s2 0 (i + 1)))
+
+val memcpy: #a:eqtype -> src:B.buffer a -> dst:B.buffer a -> len:U32.t -> Stack unit
+    (requires fun h0 ->
+        let l_src = M.loc_buffer src in
+        let l_dst = M.loc_buffer dst in
+        B.live h0 src /\ B.live h0 dst /\
+        B.length src = U32.v len /\
+        B.length dst = U32.v len /\
+        M.loc_disjoint l_src l_dst)
+    (ensures fun h0 () h1 ->
+        let l_src = M.loc_buffer src in
+        let l_dst = M.loc_buffer dst in
+        B.live h1 src /\
+        B.live h1 dst /\
+        M.(modifies l_dst h0 h1) /\
+        S.equal (B.as_seq h1 dst) (B.as_seq h0 src))
+let memcpy #a src dst len =
+    let h0 = ST.get () in
+    let inv h (i: nat) =
+        B.live h src /\ B.live h dst /\
+        M.(modifies (loc_buffer dst) h0 h) /\
+        i <= U32.v len /\
+        S.equal (Seq.slice (B.as_seq h src) 0 i) (Seq.slice (B.as_seq h dst) 0 i)
+    in
+    let body (i: U32.t{ 0 <= U32.v i /\ U32.v i < U32.v len }): Stack unit
+        (requires (fun h -> inv h (U32.v i)))
+        (ensures (fun h0 () h1 -> inv h0 (U32.v i) /\ inv h1 (U32.v i + 1)))
+=
+    let open B in
+    dst.(i) <- src.(i) in
+    C.Loops.for 0ul len inv body
+
+noextract inline_for_extraction let key_length = 32ul
+noextract inline_for_extraction let nonce_length = 24ul
+noextract inline_for_extraction let host_length = 6ul
+
+noextract inline_for_extraction let state_length = U32.(key_length +^ nonce_length +^ host_length)
+
+noextract inline_for_extraction let cipher_header_length = U32.(16ul +^ nonce_length)
+
+noextract inline_for_extraction let state1_A_length = U32.(key_length +^ host_length +^ nonce_length)
+noextract inline_for_extraction let state2_A_length = key_length
+noextract inline_for_extraction let state_B_length = U32.(key_length +^ nonce_length)
+
+noextract inline_for_extraction let message1_length = U32.(host_length +^ host_length +^ nonce_length)
+noextract inline_for_extraction let message3_length = U32.(cipher_header_length +^ key_length +^ host_length)
+noextract inline_for_extraction let message2_length = U32.(cipher_header_length +^ nonce_length +^ key_length +^ host_length +^ message3_length)
+noextract inline_for_extraction let message4_length = U32.(cipher_header_length +^ nonce_length)
+noextract inline_for_extraction let message5_length = U32.(cipher_header_length +^ nonce_length)
+
+noextract inline_for_extraction type key   = b: B.buffer U8.t{B.length b = U32.v key_length}
+noextract inline_for_extraction type host  = b: B.buffer U8.t{B.length b = U32.v host_length}
+noextract inline_for_extraction type nonce = b: B.buffer U8.t{B.length b = U32.v nonce_length}
+
+noextract inline_for_extraction type state1_At = b: B.buffer U8.t{B.length b = U32.v state1_A_length}
+noextract inline_for_extraction type state2_At = b: B.buffer U8.t{B.length b = U32.v state2_A_length}
+noextract inline_for_extraction type state_Bt  = b: B.buffer U8.t{B.length b = U32.v state_B_length}
+
+noextract inline_for_extraction type m1t = b: B.buffer U8.t{B.length b = U32.v message1_length}
+noextract inline_for_extraction type m3t = b: B.buffer U8.t{B.length b = U32.v message3_length}
+noextract inline_for_extraction type m2t = b: B.buffer U8.t{B.length b = U32.v message2_length}
+noextract inline_for_extraction type m4t = b: B.buffer U8.t{B.length b = U32.v message4_length}
+noextract inline_for_extraction type m5t = b: B.buffer U8.t{B.length b = U32.v message5_length}
+
+assume val new_key: (r: key) -> EXT unit
+assume val new_host: (r: host) -> EXT unit
+assume val new_nonce: (r: nonce) -> EXT unit
+
+effect Mem (a: Type) (b: B.buffer U8.t) = Stack a
+    (requires fun h -> B.live h b)
+    (ensures  fun h0 _ h1 -> ST.modifies_none h0 h1)
+
+noextract let fst (l1, l2, l3: (S.seq 'a & S.seq 'a & S.seq 'a))
+    = l1
+
+noextract let snd (l1, l2, l3: (S.seq 'a & S.seq 'a & S.seq 'a))
+    = l2
+
+noextract let join3 (l1, l2, l3: (S.seq 'a & S.seq 'a & S.seq 'a))
+    = S.(l1 @| l2 @| l3)
+
+noextract inline_for_extraction let lena = 1ul
+noextract inline_for_extraction let lenb = U32.(lena +^ lena +^ lena)
+
+let foo (b: B.buffer U8.t{B.length b = U32.v lenb}) (a: B.buffer U8.t{B.length a = U32.v lena}): Stack unit
+    (requires fun h ->
+        B.live h a /\
+        B.live h b /\
+        B.disjoint a b /\
+        True)
+    (ensures  fun h0 _ h1 ->
+        M.modifies (M.loc_buffer b) h0 h1 /\
+        // S.slice (B.as_seq h1 b) 0 1 `S.equal` (B.as_seq h1 a) /\
+        B.as_seq h1 b `S.equal` S.((B.as_seq h1 a) @| (B.as_seq h1 a) @| (B.as_seq h1 a)) /\
+        True)
+=
+    memcpy a (B.sub b 0ul lena) lena;
+    memcpy a (B.sub b lena lena) lena;
+    memcpy a (B.sub b U32.(lena+^lena) lena) lena;
+    ()
+
+
+// TODO: How to prove this fully?
+let initiate_A (kAS: key) (a b: host) (nA: nonce) (state: state1_At) (m1: m1t): Stack unit
+    (requires fun h ->
+        let open B in
+        live h kAS /\ live h a /\ live h b /\ live h nA /\
+        live h state /\ live h m1 /\
+        disjoint state kAS /\ disjoint state a /\ disjoint state b /\ disjoint state nA /\
+        disjoint m1 kAS /\ disjoint m1 a /\ disjoint m1 b /\ disjoint m1 nA /\
+        disjoint state m1)
+    (ensures  fun h0 _ h1 ->
+        let open M in
+        let state', m1' = Spec.initiate_A (B.as_seq h0 kAS) (B.as_seq h0 a) (B.as_seq h0 b) (B.as_seq h0 nA) in
+        modifies (loc_union (loc_buffer state) (loc_buffer m1)) h0 h1 /\
+        B.as_seq h1 state `S.equal` join3 state' /\
+        // B.as_seq h1 m1 `S.equal` join3 m1' /\
+        True)
+=
+    let open U32 in
+    let h0 = ST.get() in
+    // state
+    memcpy kAS (B.sub state 0ul key_length) key_length;
+    memcpy b   (B.sub state key_length host_length) host_length;
+    memcpy nA  (B.sub state (key_length +^ host_length) nonce_length) nonce_length;
+    let h1 = ST.get() in
+    // m1
+    memcpy a  (B.sub m1 0ul host_length) host_length;
+    memcpy b  (B.sub m1 host_length host_length) host_length;
+    memcpy nA (B.sub m1 (host_length +^ host_length) nonce_length) nonce_length;
+    let h2 = ST.get() in
+    let _ = assert M.(modifies (loc_buffer state) h0 h1) in
+    let _ = assert M.(modifies (loc_buffer m1) h1 h2) in
+    let state', m1' = Spec.initiate_A (B.as_seq h0 kAS) (B.as_seq h0 a) (B.as_seq h0 b) (B.as_seq h0 nA) in
+    let _ = assert (B.as_seq h2 state `S.equal` join3 state') in
+    // let _ = assert (B.as_seq h2 m1 `S.equal` join3 m1') in
+    ()
+
+noextract inline_for_extraction let nul = (U8.uint_to_t 0)
+
+noextract let test (kAS: Spec.key) (a b: Spec.host) (nA: Spec.nonce): St unit =
+    push_frame();
+    let m1 = B.alloca nul message1_length in
+    let state = B.alloca nul state1_A_length in
+    pop_frame()
