Makefile
@@ -1,13 +1,39 @@
 .PHONY: clean all
 
-IMPL_SRCS=Test.fst
-SPEC_SRCS=$(IMPL_SRCS) fstar/Spec.NeedSchr.fst
+FSTAR_HOME ?= $(HOME)/everest/FStar
+KREMLIN_HOME ?= $(HOME)/everest/kremlin
+HACL_STAR ?= $(HOME)/everest/hacl-star
 
-OCAML_SRCS=dist/spec/Test.ml dist/spec/Spec_NeedSchr.ml
-GENC_SRCS=dist/impl/Test.c
+FSTAR ?= $(FSTAR_HOME)/bin/fstar.exe
+KRML ?= $(KREMLIN_HOME)/krml
+
+SPEC_SRCS=fstar/Spec.NeedSchr.fst
+IMPL_SRCS=fstar/Impl.NeedSchr.fst
+
+OCAML_SRCS=dist/spec/Spec_NeedSchr.ml
+GENC_SRCS=dist/impl/Impl_NeedSchr.c
 C_SRCS=$(GENC_SRCS) main.c
 
-all: $(OCAML_SRCS) out/main
+INCLUDE_DIRS=-I"$(KREMLIN_HOME)/include"
+INCLUDE_DIRS+= -I"$(KREMLIN_HOME)/kremlib/dist/minimal"
+INCLUDE_DIRS+= -I$(HACL_STAR)/dist/gcc-compatible
+
+LIBRARIES=$(KREMLIN_HOME)/kremlib/dist/generic/libkremlib.a
+LIBRARIES+= $(HACL_STAR)/dist/gcc-compatible/libevercrypt.a
+LIBRARIES+= -I.
+
+FSTAR_INCLUDES=--include $(KREMLIN_HOME)/kremlib
+FSTAR_INCLUDES+= --include fstar
+# FSTAR_INCLUDES+= --include $(HACL_STAR)/specs/lemmas
+# FSTAR_INCLUDES+= --include $(HACL_STAR)/code/bignum
+# FSTAR_INCLUDES+= --include $(HACL_STAR)/code/meta
+# FSTAR_INCLUDES+= --include $(HACL_STAR)/code/poly1305
+# FSTAR_INCLUDES+= --include $(HACL_STAR)/code/curve25519
+# FSTAR_INCLUDES+= --include $(HACL_STAR)/code/salsa20
+# FSTAR_INCLUDES+= --include $(HACL_STAR)/code/nacl-box
+# FSTAR_INCLUDES+= --include $(HACL_STAR)/lib
+
+all: $(OCAML_SRCS) dist/impl/main
 
 clean:
 	rm -rf dist
@@ -16,13 +42,13 @@ dist:
 	mkdir dist
 
 $(OCAML_SRCS): $(SPEC_SRCS) dist
-	fstar $(SPEC_SRCS) --codegen OCaml --odir dist/spec --include $(KREMLIN_HOME)/kremlib
+	$(FSTAR) $(SPEC_SRCS) --codegen OCaml --odir dist/spec
 
-dist/impl/out.krml: $(IMPL_SRCS) dist
-	fstar $(IMPL_SRCS) --codegen Kremlin --odir dist/impl --include $(KREMLIN_HOME)/kremlib
+dist/impl/out.krml: $(IMPL_SRCS) $(SPEC_SRCS) dist
+	$(FSTAR) $(IMPL_SRCS) --codegen Kremlin --odir dist/impl $(FSTAR_INCLUDES)
 
 $(GENC_SRCS): dist/impl/out.krml
-	krml -tmpdir dist/impl -skip-compilation dist/impl/out.krml
+	$(KRML) -tmpdir dist/impl -skip-compilation -skip-makefiles dist/impl/out.krml -add-include "<header.h>"
 
-out/main: $(C_SRCS)
-	gcc -I"$(KREMLIN_HOME)/include" -I"$(KREMLIN_HOME)/kremlib/dist/minimal" $(C_SRCS) -o dist/main $(KREMLIN_HOME)/kremlib/dist/generic/libkremlib.a
+dist/impl/main: $(C_SRCS) header.h
+	gcc $(INCLUDE_DIRS) $(C_SRCS) -o dist/impl/main $(LIBRARIES) -O3
